src/Concurrent/BarbedBisim.v
@@ -105,9 +105,9 @@ match p with
     fold_right (fun x acc => usedPIDsVal x ++ acc) [] mb.1 ++
     fold_right (fun x acc => usedPIDsVal x ++ acc) [] mb.2
 | inr links => (* TODO: should links should be considered? - Probably *)
-    fold_right (fun x acc => x.1::usedPIDsVal x.2 ++ acc) [] links
+    fold_right (fun x acc => (x.1::usedPIDsVal x.2) ++ acc) [] links
 end.
-
+Print usedPIDsProc.
 (* Definition isUsed (ι : PID) (Π : ProcessPool) : Prop :=
   exists ι' p, Π ι' = Some p /\ In ι (usedPidsProc p). *)
 
